complete Monads intro

Firstproject/Monads.lean
@@ -1,3 +1,5 @@
+namespace Maybe
+
 def first (xs : List α) : Option α :=
   xs[0]?
 
@@ -58,7 +60,9 @@ def firstThirdFifthSeventh'' (xs : List α) : Option (α × α × α × α) :=
   xs[6]? ~~> fun seventh =>
   some (first, third, fifth, seventh)
 
-namespace Handling
+end Maybe
+
+namespace Exception
 
 -- Lean's equivalent of OCaml's [('a,'e) Result]
 inductive Except (ε : Type) (α : Type) where
@@ -92,8 +96,8 @@ def firstThirdBad (xs : List α) : Except String (α × α) :=
                     | Except.error msg => Except.error msg
                     | Except.ok x2 => Except.ok (x0, x2)
 
-def andThen (e : Except ε α) (next : α -> Except ε β) : Except ε β :=
-  match e with
+def andThen (attempt : Except ε α) (next : α -> Except ε β) : Except ε β :=
+  match attempt with
   | Except.error msg => Except.error msg
   | Except.ok x => next x
 
@@ -124,8 +128,257 @@ def firstThirdFifthSeventh (xs : List α) : Except String (α × α × α × α)
 #eval firstThirdFifthSeventh
 ediblePlants
 
-end Handling
+end Exception
 
 namespace Logging
 
+def isEven (i : Int) : Bool :=
+  i % 2 == 0
+
+  def sumAndFindEvens : List Int → List Int × Int
+  | [] => ([], 0)
+  | x :: xs =>
+    let (ys, sum) := sumAndFindEvens xs
+    (if isEven x then x :: ys else ys, sum + x)
+
+#eval sumAndFindEvens [0,2,4,6,8,10]
+#eval sumAndFindEvens [0,1,2,4,7,6,1,21]
+
+inductive BinTree (α : Type) where
+  | leaf : BinTree α
+  | branch : BinTree α -> α -> BinTree α -> BinTree α
+deriving Repr
+
+def inorderSum : BinTree Int → List Int × Int
+  | BinTree.leaf => ([], 0)
+  | BinTree.branch l v r =>
+    let (nodesL, sumL) := inorderSum l
+    let (hereVisited, hereSum) := ([v], v)
+    let (nodesR, sumR) := inorderSum r
+    (nodesL ++ hereVisited ++ nodesR, sumL + hereSum + sumR)
+
+open BinTree
+def tree : BinTree Int :=
+  branch
+    (branch leaf 2 leaf)
+    1
+    (branch
+      (branch leaf 3
+        (branch leaf 5 leaf))
+      4
+      leaf)
+
+#eval inorderSum tree
+
+-- Making the pattern more evident
+def sumAndFindEvens' : List Int → List Int × Int
+  | [] => ([], 0)
+  | x :: xs =>
+    let (moreEvens, sum) := sumAndFindEvens xs
+    let (evenHere, ()) := (if isEven x then [x] else [], ())
+    (evenHere ++ moreEvens, sum + x)
+    /- Append the nodes currently available to the nodes accumulated so far,
+       calculate the function's result using the information currently and
+       the other information carried over -/
+
+-- Pair of accumulated result and value
+structure WithLog (logged : Type) (α : Type) where
+  log : List logged
+  val : α
+deriving Repr
+
+-- ~10 min
+def andThenUgly (result : WithLog Λ α) (next : α → WithLog Λ β) : WithLog Λ β :=
+  let result' := next result.val
+  {
+    log := result.log ++ result'.log
+    val := result'.val
+  }
+
+def andThen (result : WithLog Λ α) (next : α → WithLog Λ β) : WithLog Λ β :=
+  let {log := thisOut, val := thisVal} := result
+  let {log := nextOut, val := nextVal} := next thisVal
+  {log := thisOut ++ nextOut, val := nextVal}
+
+def ok (x : β) : WithLog α β := {log := [], val := x}
+
+def save (data : α) : WithLog α Unit := {log := [data], val := ()}
+
+-- ~18 min
+def sumAndFindEvens'' : List Int → WithLog Int Int
+  | [] => ok 0
+  | x :: xs =>
+    -- Inverting the order of the two lines inverts the order of the log (try it!). The sum, of course, stays the same
+    andThen (sumAndFindEvens'' xs)                fun sum =>
+    andThen (if isEven x then save x else ok ())  fun () =>
+    ok (x + sum)
+
+#eval sumAndFindEvens [0,2,4,6,8,10]
+#eval sumAndFindEvens [0,1,2,4,7,6,1,21]
+
+#eval sumAndFindEvens'' [0,2,4,6,8,10]
+#eval sumAndFindEvens'' [0,1,2,4,7,6,1,21]
+
+-- ~5 min
+def inorderSum' : BinTree Int → WithLog Int Int
+  | BinTree.leaf => ok 0
+  | BinTree.branch l v r =>
+    andThen (inorderSum' l) fun leftSum =>
+    andThen (save v)        fun () =>
+    andThen (inorderSum' r) fun rightSum =>
+    ok (leftSum + v + rightSum)
+
+#eval inorderSum tree
+#eval inorderSum' tree
+
+-- [inorderSum] logs the left branch first then the root and finally the right branch
+def tree2 : BinTree Int :=
+  branch
+    (branch
+      (branch
+        (branch
+          (branch leaf 0 leaf)
+          1
+          leaf)
+        2
+        leaf)
+      3
+      (branch leaf (-3) leaf))
+    4
+    (branch leaf 5 leaf)
+
+#eval inorderSum' tree2
+
+infixl:55 " ~~> " => andThen
+
+def sumAndFindEvens''' : List Int → WithLog Int Int
+  | [] => ok 0
+  | x :: xs =>
+    (if isEven x then save x else ok ())
+    ~~> fun () => (sumAndFindEvens''' xs)
+    ~~> fun sum => ok (sum + x)
+
+def inorderSum'' : BinTree Int → WithLog Int Int
+  | BinTree.leaf => ok 0
+  | BinTree.branch l v r =>
+    inorderSum'' l ~~> fun leftSum =>
+    save v         ~~> fun () =>
+    inorderSum'' r ~~> fun rightSum =>
+    ok (leftSum + v + rightSum)
+
+#eval sumAndFindEvens''' [0,2,4,6,8,10]
+#eval sumAndFindEvens''' [0,1,2,4,7,6,1,21]
+#eval inorderSum'' tree2
+
+def aTree :=
+  branch
+    (branch
+      (branch leaf "a" (branch leaf "b" leaf))
+      "c"
+      leaf)
+    "d"
+    (branch leaf "e" leaf)
+
+-- Get the rightmost value in the tree
+def descendRight (t : BinTree α) : Option α :=
+  let rec helper (acc : Option α) (t' : BinTree α) :=
+    match t' with
+    | leaf => acc
+    | branch _ v r => helper (some v) r
+  match t with
+  | leaf => none
+  | branch _ v r => helper v r
+
+#eval descendRight tree
+#eval descendRight tree2
+#eval descendRight aTree
+
+-- # Numbering a tree in an inorder fashion
+
+/- First attempt:
+def tryNumbering : BinTree Int -> BinTree (Nat × Int)
+  | leaf => leaf
+  | branch l v r =>
+    Maybe.andThen (tryNumbering l |> descendRight) fun (leftMax, _) =>
+    Abort -- stuck... (bad approach) -/
+
+-- ~20 min
+def number (t : BinTree α) : BinTree (Nat × α) :=
+  let rec helper (num : Nat) (t : BinTree α) : (Nat × BinTree (Nat × α)) :=
+    match t with
+    | leaf => (num, leaf)
+    | branch l v r =>
+      let (numLeft, numberedLeft) := helper num l
+      let numThis := numLeft
+      let (numRight, numberedRight) := helper (numThis + 1) r
+      (numRight, branch numberedLeft (numThis, v) numberedRight)
+  (helper 0 t).snd
+
+#eval number aTree
+#eval number tree
+#eval number tree2
+
+-- ## Stateful computations
+
+namespace Stateful
+
+/- The thing we want to propagate now is a [State] for a single mutable
+   variable, whose values are functions.
+   These functions take an input state and return an output state together
+   with a value. Reading preserves the state, whereas writing replaces it
+   with a new one. -/
+def State (σ : Type) (α : Type) : Type :=
+  σ → (σ × α)
+
+def ok (x : α) : State σ α :=
+  fun s => (s, x)
+
+def get : State σ σ :=
+  fun s => (s, s)
+
+def set (x : σ) : State σ Unit :=
+  fun _ => (x, ())
+
+-- Sequencing of stateful operations (~10 min)
+def andThen (first : State σ α) (next : α -> State σ β) : State σ β :=
+  fun s0 =>
+    let (s1, a) : σ × α := first s0
+    let S : State σ β := next a
+    S s1
+
+infixl:55 " ~~> " => andThen
+
+-- ~52 min, peeked a lot
+def number (t : BinTree α) : BinTree (Nat × α) :=
+  let rec helper : BinTree α → State Nat (BinTree (Nat × α))
+    | leaf => ok leaf -- Base state
+    | branch l v r =>
+      helper l        ~~> fun numberedLeft =>
+      get             ~~> fun numL =>
+      set (numL + 1)  ~~> fun () =>
+      helper r        ~~> fun numberedRight =>
+      ok (branch numberedLeft (numL, v)  numberedRight)
+  (helper t 0).snd
+  /-  I'm embarassed of this attempt
+      let f :=
+        set 0 ~~> fun () =>
+        ok t  ~~> helper
+              ~~> fun numbered =>
+        ok numbered -- How do I escape from a [State]!?
+      f 0 -/
+
+#eval number tree
+#eval number aTree
+
+end Stateful
+
 end Logging
+
+
+-- Use a single element to represent the one element word
+instance : Coe α (List α) where
+  coe a := [a]
+
+example : Option Nat := List.get? (1 : Nat) 42
+example : Option Char := List.get? 'a' 42
+example : Option Bool := List.get? true 0
